json: Finish unicode encoding and decoding

src/Math.dfy
@@ -28,8 +28,137 @@ module Math {
     if a >= 0 then a else -a
   }
 
-  function method {:opaque} IntPow(x: int, n: nat) : int {
+  function method {:opaque} IntPow(base: int, n: nat): int {
     if n == 0 then 1
-    else x * IntPow(x, n - 1)
+    else base * IntPow(base, n - 1)
   }
+
+  function method {:opaque} IntLog(base: nat, pow: nat): nat
+    requires base > 1
+    decreases pow
+    // TODO: pow > 0 ==> IntPow(base, IntLog(base, pow)) <= pow < IntPow(base, IntLog(base, pow) + 1)
+  {
+    if pow < base then 0
+    else
+      assert pow < pow * base; assert pow / base < pow;
+      1 + IntLog(base, pow / base)
+  }
+
+  lemma {:induction false} Divide_Increasing(base: nat, pow: nat, pow': nat)
+    requires base > 1
+    requires pow <= pow'
+    ensures pow / base <= pow' / base
+  {
+    var q, q', r, r' := pow / base, pow' / base, pow % base, pow' % base;
+    assert pow == q * base + r;
+    assert pow' == q' * base + r';
+    assert 0 <= r < base && 0 <= r' < base;
+    var dp, dq, dr := pow' - pow, q' - q, r' - r;
+    assert dp == dq * base + dr;
+    if dq < 0 {
+      assert dq * base < -base;
+      assert dr <= base;
+      assert dp == dq * base + dr < 0;
+      assert false;
+    }
+  }
+
+  lemma {:induction false} IntLog_Increasing(base: nat, pow: nat, pow': nat)
+    requires base > 1
+    requires pow <= pow'
+    ensures IntLog(base, pow) <= IntLog(base, pow')
+    decreases pow
+  {
+    reveal IntLog();
+    if pow' < base {
+      assert IntLog(base, pow) == 0 == IntLog(base, pow');
+    } else if pow < base {
+      assert IntLog(base, pow) == 0;
+    } else {
+      assert pow < pow * base; assert pow / base < pow;
+      assert pow' < pow' * base; assert pow' / base < pow';
+      assert pow / base <= pow' / base by { Divide_Increasing(base, pow, pow'); }
+      IntLog_Increasing(base, pow / base, pow' / base);
+    }
+  }
+
+  // lemma {:induction n} IntPow_Nat(base: nat, n: nat)
+  //   ensures IntPow(base, n) >= 0
+  // {
+  //   reveal IntPow();
+  // }
+
+  // lemma {:induction n} IntPow_NonZero(base: int, n: nat)
+  //   requires base != 0
+  //   ensures IntPow(base, n) != 0
+  // {
+  //   reveal IntPow();
+  // }
+
+  // function method {:opaque} NatPow(base: nat, n: nat): nat {
+  //   IntPow_Nat(base, n);
+  //   IntPow(base, n)
+  // }
+
+  // lemma {:induction false} NatPow_NonZero(base: nat, n: nat)
+  //   requires base != 0
+  //   ensures NatPow(base, n) != 0
+  // {
+  //   reveal NatPow(); IntPow_NonZero(base, n);
+  // }
+
+  // function method {:opaque} IntLogSup(base: nat, pow: nat): (log: nat)
+  //   requires base > 1
+  //   ensures log > 0
+  //   decreases pow
+  //   // IntPow(base, IntLogSup(base, pow) - 1) - 1 <= pow <= IntPow(base, IntLogSup(base, pow))
+  // {
+  //   if pow < base then 1
+  //   else
+  //     assert pow < pow * base;
+  //     assert pow / base < pow;
+  //     1 + IntLog(base, pow / base)
+  // }
+
+  // // lemma {:induction false} IntLogSup_transfer(base: nat, n: nat, n': nat)
+  // //   requires base > 1
+  // //   requires n > n'
+  // //   ensures
+  // //     (NatPow_NonZero(base, n); NatPow_NonZero(base, n');
+  // //      IntLogSup(base, NatPow(base, n), NatPow(base, n')) == IntLogSup(base, NatPow(base, n - n')))
+  // // {
+  // //   reveal NatPow();
+  // //   reveal IntPow();
+  // //   reveal IntLogSup();
+  // //   if n' == 0 {
+  // //   } else {
+  // //     NatPow_NonZero(base, n); NatPow_NonZero(base, n'); NatPow_NonZero(base, n' - 1);
+  // //     calc {
+  // //       IntLogSup(base, NatPow(base, n), NatPow(base, n'));
+  // //       1 + IntLogSup(base, NatPow(base, n), NatPow(base, n' - 1) * base) - 1;
+  // //       { assume NatPow(base, n) > NatPow(base, n'); } // FIXME wrong
+  // //       IntLogSup(base, NatPow(base, n), NatPow(base, n' - 1)) - 1;
+  // //       { IntLogSup_transfer(); }
+  // //       IntLogSup(base, NatPow(base, n - n'))
+  // //     }
+  // //   }
+  // // }
+
+  // lemma {:induction false} IntPow_IntLogSup(base: nat, n: nat)
+  //   requires base > 1
+  //   ensures IntLogSup(base, NatPow(base, n)) - 1 < n <= IntLogSup(base, NatPow(base, n))
+  // {
+  //   reveal IntLogSup();
+  //   reveal IntPow();
+  //   reveal NatPow();
+  //   if n == 0 {
+  //   } else {
+  //     calc {
+  //       IntLogSup(base, NatPow(base, n));
+  //       IntLogSup(base, NatPow(base, n - 1) * base);
+  //       IntLogSup(base, NatPow(base, n - 1) * base);
+  //       1 + IntLogSup(base, NatPow(base, n - 1));
+  //     }
+  //   }
+  // }
 }
