src/JSON/JSON.API.dfy
@@ -2,9 +2,12 @@ include "JSON.Errors.dfy"
 include "JSON.Grammar.dfy"
 include "JSON.Spec.dfy"
 include "JSON.Serializer.dfy"
-include "JSON.ZeroCopy.Serializer.dfy"
+include "JSON.Deserializer.dfy"
+include "JSON.ZeroCopy.API.dfy"
 
 module {:options "/functionSyntax:4"} JSON.API {
+  // TODO: Propagate proofs
+
   import opened BoundedInts
   import opened Wrappers
   import Vs = Views.Core
@@ -13,41 +16,31 @@ module {:options "/functionSyntax:4"} JSON.API {
   import opened AST
   import Spec
   import S = Serializer
-  import ZS = ZeroCopy.Serializer
-  // import Deserializer
+  import DS = Deserializer
+  import ZAPI = ZeroCopy.API
 
   function {:opaque} Serialize(js: JSON) : (bs: SerializationResult<seq<byte>>)
-    // TODO: Carry proofs all the way
-    // ensures bs.Success? ==> bs.value == Spec.JSON(js)
   {
     var js :- S.JSON(js);
-    Success(ZS.Text(js).Bytes())
+    Success(ZAPI.Serialize(js))
   }
 
   method SerializeAlloc(js: JSON) returns (bs: SerializationResult<array<byte>>)
-    // TODO: Carry proofs all the way
-    // ensures bs.Success? ==> fresh(bs.value)
-    // ensures bs.Success? ==> bs.value[..] == Spec.JSON(js)
   {
     var js :- S.JSON(js);
-    bs := ZS.Serialize(js);
+    bs := ZAPI.SerializeAlloc(js);
   }
 
   method SerializeBlit(js: JSON, bs: array<byte>) returns (len: SerializationResult<uint32>)
     modifies bs
-    // TODO: Carry proofs all the way
-    // ensures len.Success? ==> len.value as int <= bs.Length
-    // ensures len.Success? ==> bs[..len.value] == Spec.JSON(js)
-    // ensures len.Success? ==> bs[len.value..] == old(bs[len.value..])
-    // ensures len.Failure? ==> unchanged(bs)
   {
     var js :- S.JSON(js);
-    len := ZS.SerializeTo(js, bs);
+    len := ZAPI.SerializeBlit(js, bs);
   }
 
-  // function {:opaque} Deserialize(bs: seq<byte>) : (js: Result<JSON, Deserializer.Error>)
-  //   ensures js.Success? ==> bs == Spec.JSON(js.value)
-  // {
-  //   Deserializer.API.OfBytes(bs)
-  // }
+  function {:opaque} Deserialize(bs: seq<byte>) : (js: DeserializationResult<JSON>)
+  {
+    var js :- ZAPI.Deserialize(bs);
+    DS.JSON(js)
+  }
 }
