src/JSON/JSON.Errors.dfy
@@ -1,24 +1,39 @@
 include "../Wrappers.dfy"
+include "../BoundedInts.dfy"
+include "Str.dfy"
 
 module {:options "/functionSyntax:4"} JSON.Errors {
   import Wrappers
+  import opened BoundedInts
+  import Str
 
   datatype DeserializationError =
     | UnterminatedSequence
-    | UnsupportedEscape
+    | UnsupportedEscape(str: string)
     | EscapeAtEOS
     | EmptyNumber
     | ExpectingEOF
     | IntOverflow
+    | ReachedEOF
+    | ExpectingByte(expected: byte, b: opt_byte)
+    | ExpectingAnyByte(expected_sq: seq<byte>, b: opt_byte)
   {
     function ToString() : string {
       match this
         case UnterminatedSequence => "Unterminated sequence"
-        case UnsupportedEscape => "Unsupported escape sequence"
+        case UnsupportedEscape(str) => "Unsupported escape sequence: " + str
         case EscapeAtEOS => "Escape character at end of string"
         case EmptyNumber => "Number must contain at least one digit"
         case ExpectingEOF => "Expecting EOF"
         case IntOverflow => "Input length does not fit in a 32-bit counter"
+        case ReachedEOF => "Reached EOF"
+        case ExpectingByte(b0, b) =>
+          var c := if b > 0 then "'" + [b as char] + "'" else "EOF";
+          "Expecting '" + [b0 as char] + "', read " + c
+        case ExpectingAnyByte(bs0, b) =>
+          var c := if b > 0 then "'" + [b as char] + "'" else "EOF";
+          var c0s := seq(|bs0|, idx requires 0 <= idx < |bs0| => bs0[idx] as char);
+          "Expecting one of '" + c0s + "', read " + c
     }
   }
 
@@ -26,6 +41,14 @@ module {:options "/functionSyntax:4"} JSON.Errors {
     | OutOfMemory
     | IntTooLarge(i: int)
     | StringTooLong(s: string)
+  {
+    function ToString() : string {
+      match this
+        case OutOfMemory => "Out of memory"
+        case IntTooLarge(i: int) => "Integer too large: " + Str.OfInt(i)
+        case StringTooLong(s: string) => "String too long: " + s
+    }
+  }
 
   type SerializationResult<+T> = Wrappers.Result<T, SerializationError>
   type DeserializationResult<+T> = Wrappers.Result<T, DeserializationError>
