src/JSON/JSON.Spec.dfy
@@ -20,16 +20,49 @@ module {:options "/functionSyntax:4"} JSON.Spec {
 
   type bytes = seq<uint8>
 
+  function EscapeUnicode(c: uint16): string {
+    var s := Str.OfNat(c as nat, 16);
+    assert |s| <= 4 by {
+      assert c as nat <= 0xFFFF;
+      assert Math.IntLog(16, c as nat) <= Math.IntLog(16, 0xFFFF) by {
+        Math.IntLog_Increasing(16, c as nat, 0xFFFF);
+      }
+      assert Math.IntLog(16, 0xFFFF) == 3 by { reveal Math.IntLog(); }
+    }
+    s + seq(4 - |s|, _ => ' ')
+  }
+
+  function Escape(str: string, start: nat := 0): string
+    decreases |str| - start
+  {
+    if start >= |str| then []
+    else
+      (match str[start] as uint16
+         case 0x22 => "\\\"" // quotation mark
+         case 0x5C => "\\\\"  // reverse solidus
+         case 0x08 => "\\b"  // backspace
+         case 0x0C => "\\f"  // form feed
+         case 0x0A => "\\n"  // line feed
+         case 0x0D => "\\r"  // carriage return
+         case 0x09 => "\\t"  // tab
+         case c =>
+           if c < 0x001F then "\\u" + EscapeUnicode(c)
+           else [str[start]])
+      + Escape(str, start + 1)
+  }
+
   function String(str: string): bytes {
-    Str.ToBytes("'") + Transcode16To8(Str.EscapeQuotes(str)) + Str.ToBytes("'")
+    Str.ToBytes("\"") + Transcode16To8(Escape(str)) + Str.ToBytes("\"")
   }
 
   function Number(dec: Decimal): bytes {
-    Transcode16To8(Str.OfInt(dec.n)) + Str.ToBytes("e") + Transcode16To8(Str.OfInt(dec.e10))
+    Transcode16To8(Str.OfInt(dec.n)) +
+      (if dec.e10 == 0 then []
+       else Str.ToBytes("e") + Transcode16To8(Str.OfInt(dec.e10)))
   }
 
   function KV(kv: (string, JSON)): bytes {
-    String(kv.0) + Str.ToBytes(", ") + JSON(kv.1)
+    String(kv.0) + Str.ToBytes(":") + JSON(kv.1)
   }
 
   function Join(sep: bytes, items: seq<bytes>): bytes {
