src/NonlinearArithmetic/Power.dfy
@@ -12,12 +12,14 @@
 former takes arguments and may be more stable and less reliant on Z3
 heuristics. The latter includes automation and its use requires less effort */
 
+include "../Math.dfy"
 include "DivMod.dfy"
 include "Internals/GeneralInternals.dfy"
 include "Mul.dfy"
 include "Internals/MulInternals.dfy"
 
 module Power {
+  import Math
   import opened DivMod
   import opened GeneralInternals
   import opened Mul
@@ -25,7 +27,9 @@ module Power {
 
   function method {:opaque} Pow(b: int, e: nat): int
     decreases e
+    ensures Pow(b, e) == Math.IntPow(b, e)
   {
+    reveal Math.IntPow();
     if e == 0 then
       1
     else
